src/main/scala/viper/carbon/modules/impls/QuantifiedPermModule.scala
@@ -30,7 +30,7 @@ import viper.carbon.boogie.Assert
 import viper.carbon.boogie.ConstDecl
 import viper.carbon.boogie.Const
 import viper.carbon.boogie.LocalVar
-import viper.silver.ast.{LocationAccess, PermMul, PredicateAccess, PredicateAccessPredicate, ResourceAccess, WildcardPerm, SWildcardPerm}
+import viper.silver.ast.{LocationAccess, PermMul, PredicateAccess, PredicateAccessPredicate, ResourceAccess, WildcardPerm}
 import viper.carbon.boogie.Forall
 import viper.carbon.boogie.Assign
 import viper.carbon.boogie.Func
@@ -73,12 +73,12 @@ class QuantifiedPermModule(val verifier: Verifier)
 
   implicit val namespace = verifier.freshNamespace("perm")
   private val axiomNamespace = verifier.freshNamespace("perm.axiom")
-  private val pairTypeName = "Pair"
-  private val pairConstructName = Identifier("pair")
+  private val tupleTypeName = "Tuple"
+  private val tupleConstructName = Identifier("tuple")
   private val fstConstructName = Identifier("fst")
   private val sndConstructName = Identifier("snd")
-  def pairType = NamedType(pairTypeName, Seq(TypeVar("A"), TypeVar("B")))
-  def pairTypeOfPerm = NamedType(pairTypeName, Seq(Real, Bool))
+  def tupleType = NamedType(tupleTypeName, Seq(TypeVar("A"), TypeVar("B")))
+  def tupleTypeOfPerm = NamedType(tupleTypeName, Seq(Real, Bool))
   private val permTypeName = "Perm"
   private val maskTypeName = "MaskType"
   private val maskType = NamedType(maskTypeName)
@@ -107,14 +107,16 @@ class QuantifiedPermModule(val verifier: Verifier)
   private val wandMaskFieldName = Identifier("WandMaskField")
 
 
-  private val resultMask = LocalVarDecl(Identifier("ResultMask"),maskType)
-  private val summandMask1 = LocalVarDecl(Identifier("SummandMask1"),maskType)
-  private val summandMask2 = LocalVarDecl(Identifier("SummandMask2"),maskType)
+  private val resultMask = LocalVarDecl(Identifier("ResultMask"), maskType)
+  private val summandMask1 = LocalVarDecl(Identifier("SummandMask1"), maskType)
+  private val summandMask2 = LocalVarDecl(Identifier("SummandMask2"), maskType)
 
 
   // TODO: where are these identifiers needed
   private val sumMasks = Identifier("sumMask")
+  private val sumTuples = Identifier("sumTuple")
   private val tempMask = LocalVar(Identifier("TempMask"),maskType)
+
 
   private val qpMaskName = Identifier("QPMask")
   private val qpMask = LocalVar(qpMaskName, maskType)
@@ -127,65 +129,188 @@ class QuantifiedPermModule(val verifier: Verifier)
   private var inverseFuncs: ListBuffer[Func] = new ListBuffer[Func](); //list of inverse functions used for inhale/exhale qp
   private var rangeFuncs: ListBuffer[Func] = new ListBuffer[Func](); //list of inverse functions used for inhale/exhale qp
   private var triggerFuncs: ListBuffer[Func] = new ListBuffer[Func](); //list of inverse functions used for inhale/exhale qp
+  def tuple(args: Seq[viper.carbon.boogie.Exp], ret_type:Type=tupleType) : FuncApp = FuncApp(tupleConstructName, args, ret_type)
+  def fst(args: Seq[viper.carbon.boogie.Exp], ret_type:Type = TypeVar("A")): FuncApp = FuncApp(fstConstructName, args, ret_type)
+  def snd(args: Seq[viper.carbon.boogie.Exp], ret_type:Type = TypeVar("B")): FuncApp = FuncApp(sndConstructName, args, ret_type)
+  
+  def tuplePreamble = {
+    val obj = LocalVarDecl(Identifier("o")(axiomNamespace), refType)
+    val field = LocalVarDecl(Identifier("f")(axiomNamespace), fieldType)
+    val ident_a = LocalVar(Identifier("a")(axiomNamespace), TypeVar("A")) 
+    val ident_b = LocalVar(Identifier("b")(axiomNamespace), TypeVar("B"))
+    val ident_p = LocalVar(Identifier("p")(axiomNamespace), tupleType)
+    var decl_a_ax = LocalVarDecl(Identifier("a")(axiomNamespace), TypeVar("A")) 
+    var decl_b_ax = LocalVarDecl(Identifier("b")(axiomNamespace), TypeVar("B")) 
+    var decl_p_ax = LocalVarDecl(Identifier("p")(axiomNamespace), tupleType) 
+    
+    def staticTuple = tuple(Seq(ident_a, ident_b)) 
+    def staticFst = fst(staticTuple)
+    //def staticGoodMask = FuncApp(goodMaskName, LocalVar(maskName, maskType), Bool)
+    def staticSnd = snd(staticTuple)
+    def staticTupleSndFst = tuple(Seq( fst(ident_p), snd(ident_p)))
+      
+      // type Tuple A B;
+      TypeDecl(tupleType) :: 
+      // function tuple<A, B>(a: A, b: B): Tuple A B;
+      Func(tupleConstructName, Seq(decl_a_ax, decl_b_ax), tupleType) ::
+      // function fst<A, B>(p: (Tuple A B)): A;
+      Func(fstConstructName, Seq(decl_p_ax), TypeVar("A")) ::
+      // function snd<A, B>(p: (Tuple A B)): B;
+      Func(sndConstructName, Seq(decl_p_ax), TypeVar("B")) ::
+      // axiom (forall <A, B> a_1: A, b_1: B ::
+      //   { (tuple(a_1, b_1): Tuple A B) }
+      //     (fst((tuple(a_1, b_1): Tuple A B)): A) == a_1
+      //   );
+      Axiom(Forall(Seq(decl_a_ax, decl_b_ax),
+        Trigger(staticTuple),
+        staticFst === ident_a
+      )) ::
+      // axiom (forall <A, B> a_1: A, b_1: B ::
+      //   { (tuple(a_1, b_1): Tuple A B) }
+      //   (snd((tuple(a_1, b_1): Tuple A B)): B) == b_1
+      // );
+      Axiom(Forall(Seq(decl_a_ax, decl_b_ax),
+        Trigger(staticTuple),
+        staticSnd === ident_b
+      )) ::
+      // axiom (forall <A, B> p_1: (tuple A B) ::
+      //   { (fst(p_1): A) } { (snd(p_1): B) }
+      //   (Tuple((fst(p_1): A), (snd(p_1): B)): Tuple A B) == p_1
+      // );
+      Axiom(Forall(Seq(decl_p_ax),
+        // TODO: maybe add aditional trigger for tuple
+        Seq(Trigger(fst(ident_p)), Trigger(snd(ident_p))),
+        staticTupleSndFst === ident_p
+      )) :: Nil ++
+      {
+        val tupleSumResult = LocalVarDecl(Identifier("TupleSumResult")(axiomNamespace), permType) 
+        val tupleSummand1 = LocalVarDecl(Identifier("TupleSummand1")(axiomNamespace), permType)
+        val tupleSummand2 = LocalVarDecl(Identifier("TupleSummand2")(axiomNamespace), permType)
+        val args = Seq(tupleSumResult, tupleSummand1, tupleSummand2)
+        val tupleSumResult_var = LocalVar(Identifier("TupleSumResult")(axiomNamespace), permType) 
+        val tupleSummand1_var = LocalVar(Identifier("TupleSummand1")(axiomNamespace), permType)
+        val tupleSummand2_var = LocalVar(Identifier("TupleSummand2")(axiomNamespace), permType)
+        val funcApp = FuncApp(sumTuples, args map (_.l), Bool)
+        
+        // function sumTuple(ResultMask: MaskType, SummandMask1: MaskType, SummandMask2: MaskType): bool;
+        Func(sumTuples, args, Bool) :: 
+        // TODO: add ouput code
+        Axiom(Forall(
+          args,
+          Trigger(Seq(funcApp)),
+          funcApp <==> (fst(Seq(tupleSumResult_var), Real) === fst(Seq(tupleSummand1_var), Real) + fst(Seq(tupleSummand2_var), Real))
+                      && (snd(Seq(tupleSumResult_var), Bool) === snd(Seq(tupleSummand1_var), Bool) || snd(Seq(tupleSummand2_var), Bool))
+        )) :: Nil 
+      } 
+  }
 
-  override def preamble = {
+  def permPreamble = {
     val obj = LocalVarDecl(Identifier("o")(axiomNamespace), refType)
     val field = LocalVarDecl(Identifier("f")(axiomNamespace), fieldType)
     val permInZeroMask = MapSelect(zeroMask, Seq(obj.l, field.l))
-    val permInZeroPMask = MapSelect(zeroPMask, Seq(obj.l, field.l))
-    val ident_a = LocalVarDecl(Identifier("a")(axiomNamespace), TypeVar("A")) 
-    val ident_b = LocalVarDecl(Identifier("b")(axiomNamespace), TypeVar("B"))
-    val ident_p = LocalVarDecl(Identifier("p")(axiomNamespace), pairType)
-    val y = FuncApp(pairConstructName, Seq(ident_a, ident_b) map (_.l), pairType)
-    val funcAppFst = FuncApp(fstConstructName, Seq(ident_p) map (_.l), TypeVar("A"))
-    val funcAppSnd = FuncApp(sndConstructName, Seq(ident_p) map (_.l), TypeVar("B"))
-    val funcAppPairSndFst = FuncApp(pairConstructName, Seq(funcAppFst, funcAppSnd), pairType)
-    val funcAppPair = FuncApp(pairConstructName, Seq(ident_a, ident_b) map (_.l), pairType)
-    
-    // Define pair
-      // type Pair A B;
-      // function pair<A, B>(a: A, b: B) : Pair A B;
-      // function fst<A, B>(p: Pair A B) : A;
-      // function snd<A, B>(p: Pair A B) : B;
-      // axiom (forall <A, B> a:A, b:B :: {pair(a,b)} fst(pair(a,b)) == a);
-      // axiom (forall <A, B> a:A, b:B :: {pair(a,b)} snd(pair(a,b)) == b);
-      // axiom (forall <A, B> p: Pair A B :: {fst(p)}{snd(p)} pair(fst(p), snd(p)) == p)
-    //TypeAlias(permType, ) ::
-    
-    // permission type
-      //TypeAlias(permType, Real) ::
-      // mask and mask type
-      TypeDecl(pairType) ++ 
-      Func(pairConstructName, 
-        Seq(LocalVarDecl(Identifier("a"), TypeVar("A")), LocalVarDecl(Identifier("b"), TypeVar("B"))), 
-        pairType) ++
-      Func(fstConstructName, 
-        Seq(LocalVarDecl(Identifier("p"), pairType)), 
-        TypeVar("A")) ++
-      Func(sndConstructName, 
-        Seq(LocalVarDecl(Identifier("p"), pairType)), 
-        TypeVar("B")) ++
-      Axiom(Forall(Seq(LocalVarDecl(Identifier("a")(axiomNamespace), TypeVar("A")), LocalVarDecl(Identifier("b")(axiomNamespace), TypeVar("B"))),
-        Trigger(funcAppPair),
-        ( funcAppFst === LocalVar(Identifier("a")(axiomNamespace), TypeVar("A"))))
-      ) ++
-      Axiom(Forall(Seq(LocalVarDecl(Identifier("a")(axiomNamespace), TypeVar("A")), LocalVarDecl(Identifier("b")(axiomNamespace), TypeVar("B"))),
-        Trigger(funcAppPair),
-        ( funcAppSnd === LocalVar(Identifier("b")(axiomNamespace), TypeVar("B"))))
-       ) ++
-      Axiom(Forall(Seq(LocalVarDecl(Identifier("p")(axiomNamespace), pairType)),
-        Trigger(Seq(funcAppFst, funcAppSnd)),
-        (  funcAppPairSndFst === LocalVar(Identifier("p")(axiomNamespace), pairType)))
-       ) ++
-      TypeAlias(permType, pairTypeOfPerm) ++
+      // type Perm = tuple real bool;
+      TypeAlias(permType, tupleTypeOfPerm) ++
+      // type MaskType = <A, B> [Ref, Field A B]Perm;
       TypeAlias(maskType, MapType(Seq(refType, fieldType), permType, fieldType.freeTypeVars)) ++
+      // var Mask: MaskType;
       GlobalVarDecl(maskName, maskType) ++
-      // zero mask
+      // const ZeroMask: MaskType;
       ConstDecl(zeroMaskName, maskType) ++
+      // axiom (forall <A, B> o_1: Ref, f_3: (Field A B) ::
+      //   { ZeroMask[o_1, f_3] }
+      //   ZeroMask[o_1, f_3] == NoPerm
+      // );
       Axiom(Forall(
         Seq(obj, field),
         Trigger(permInZeroMask),
-        (permInZeroMask === noPerm))) ++
+        (permInZeroMask === noPerm)
+      )) ++
+      // const NoPerm: Perm;
+      ConstDecl(noPermName, permType) ++
+      // axiom fst(NoPerm) == 0.000000000 && !snd(NoPerm);
+      Axiom(permissionNo) ++
+      // const FullPerm: Perm;
+      ConstDecl(fullPermName, permType) ++
+      // axiom fst(FullPerm) == 1.000000000
+      Axiom(permissionFull) ++
+      // function Perm<A, B>(a: A, b: B): Perm;
+      // TODO: find out where this function is used
+      Func(permConstructName, Seq(LocalVarDecl(Identifier("a"), TypeVar("A")), LocalVarDecl(Identifier("b"), TypeVar("B"))), permType) ++ 
+      // function GoodMask(Mask: MaskType): bool;
+      Func(goodMaskName, LocalVarDecl(maskName, maskType), Bool) ++
+      // axiom (forall Heap: HeapType, Mask: MaskType ::
+      //   { state(Heap, Mask) }
+      //   state(Heap, Mask) ==> GoodMask(Mask)
+      // ); 
+      Axiom(Forall(stateModule.staticStateContributions(),
+        Trigger(Seq(staticGoodState)),
+        staticGoodState ==> staticGoodMask
+      )) ++
+      // axiom (forall <A, B> Mask: MaskType, o_1: Ref, f_3: (Field A B) ::
+      //   { GoodMask(Mask), Mask[o_1, f_3] }
+      //   (GoodMask(Mask) ==> fst(Mask[o_1, f_3]) >= fst(NoPerm)) && ((GoodMask(Mask) && !IsPredicateField(f_3)) && !IsWandField(f_3) ==> fst(Mask[o_1, f_3]) <= fst(FullPerm))
+      // ); 
+      { 
+        val perm = currentPermission(obj.l, field.l)
+        Axiom(Forall(staticStateContributions(true, true) ++ obj ++ field,
+          Trigger(Seq(staticGoodMask, perm)),
+          // permissions are non-negative
+          (staticGoodMask ==> ( fst(perm, Real) >= fst(noPerm, Real)) &&
+            // permissions for fields which aren't predicates or wands are smaller than 1
+            ((staticGoodMask && heapModule.isPredicateField(field.l).not && heapModule.isWandField(field.l).not) ==> fst(perm, Real) <= fst(fullPerm, Real)))
+        ))    
+      } ++
+      {
+        val args = staticMask ++ Seq(obj, field)
+        val funcApp = FuncApp(hasDirectPermName, args map (_.l), Bool)
+        val permission = currentPermission(staticMask(0).l, obj.l, field.l)
+        // function HasDirectPerm<A, B>(Mask: MaskType, o_1: Ref, f_3: (Field A B)): bool;
+        Func(hasDirectPermName, args, Bool) ++
+        // axiom (forall <A, B> Mask: MaskType, o_1: Ref, f_3: (Field A B) ::
+        //    { HasDirectPerm(Mask, o_1, f_3) }
+        //    HasDirectPerm(Mask, o_1, f_3) <==> fst(Mask[o_1, f_3]) > fst(NoPerm)
+        // );
+        Axiom(Forall(
+          staticMask ++ Seq(obj, field),
+          Trigger(funcApp),
+          funcApp <==> permissionPositive(permission)
+        ))
+      } ++ 
+      {
+        val args1 = Seq(resultMask, summandMask1, summandMask2)
+        // val args = Seq(tupleSumResult, tupleSummand1, tupleSummand2)
+        val permResult = currentPermission(resultMask.l, obj.l, field.l)
+        val permSummand1 = currentPermission(summandMask1.l,obj.l,field.l)
+        val permSummand2 = currentPermission(summandMask2.l,obj.l,field.l)
+        val args2 = Seq(permResult, permSummand1, permSummand2)
+        val funcAppMask = FuncApp(sumMasks, args1 map (_.l), Bool)
+        val funcAppTuple = FuncApp(sumTuples, args2, Bool)
+        // function sumMask(ResultMask: MaskType, SummandMask1: MaskType, SummandMask2: MaskType): bool;
+        Func(sumMasks, args1, Bool) ++
+        // axiom (forall <A, B> ResultMask: MaskType, SummandMask1: MaskType, SummandMask2: MaskType, o_1: Ref, f_3: (Field A B) ::
+        //    { sumMask(ResultMask, SummandMask1, SummandMask2), ResultMask[o_1, f_3] } 
+        //    { sumMask(ResultMask, SummandMask1, SummandMask2), SummandMask1[o_1, f_3] }
+        //    { sumMask(ResultMask, SummandMask1, SummandMask2), SummandMask2[o_1, f_3] }
+        //   sumMask(ResultMask, SummandMask1, SummandMask2) <==> sumTuple(ResultMask[o_1, f_3], SummandMask1[o_1, f_3], SummandMask2[o_1, f_3])
+        // );
+        // TODO: check triggers
+        Axiom(Forall(
+          args1 ++ Seq(obj,field),
+          Trigger(Seq(funcAppMask, permResult)) ++ 
+          Trigger(Seq(funcAppMask, permSummand1)) ++
+          Trigger(Seq(funcAppMask, permSummand2)),
+          funcAppMask <==> funcAppTuple
+        ))
+      } 
+  } 
+
+  override def preamble = {
+    tuplePreamble ++
+    permPreamble ++
+    {
+      val obj = LocalVarDecl(Identifier("o")(axiomNamespace), refType)
+      val field = LocalVarDecl(Identifier("f")(axiomNamespace), fieldType)
+      val permInZeroPMask = MapSelect(zeroPMask, Seq(obj.l, field.l))
       // pmask type
       TypeAlias(pmaskType, MapType(Seq(refType, fieldType), Bool, fieldType.freeTypeVars)) ++
       // zero pmask
@@ -201,66 +326,19 @@ class QuantifiedPermModule(val verifier: Verifier)
       Func(wandMaskFieldName,
         Seq(LocalVarDecl(Identifier("f"), predicateVersionFieldType())),
         predicateMaskFieldType) ++
-      // permission amount constants
-      ConstDecl(noPermName, permType) ++
-      Axiom(noPerm === RealLit(0)) ++
-      ConstDecl(fullPermName, permType) ++
-      Axiom(fullPerm === RealLit(1)) ++
-      // permission constructor
-      Func(permConstructName, Seq(LocalVarDecl(Identifier("a"), TypeVar("A")), LocalVarDecl(Identifier("b"), TypeVar("B"))), permType) ++ 
-      Nil ++
-      // good mask
-      Func(goodMaskName, LocalVarDecl(maskName, maskType), Bool) ++
-      Axiom(Forall(stateModule.staticStateContributions(),
-        Trigger(Seq(staticGoodState)),
-        staticGoodState ==> staticGoodMask)) ++ {
-      val perm = currentPermission(obj.l, field.l)
-      Axiom(Forall(staticStateContributions(true, true) ++ obj ++ field,
-        Trigger(Seq(staticGoodMask, perm)),
-        // permissions are non-negative
-        (staticGoodMask ==> ( perm >= noPerm &&
-          // permissions for fields which aren't predicates are smaller than 1
-          // permissions for fields which aren't predicates or wands are smaller than 1
-          ((staticGoodMask && heapModule.isPredicateField(field.l).not && heapModule.isWandField(field.l).not) ==> perm <= fullPerm )))
-      ))    } ++  {
-      val obj = LocalVarDecl(Identifier("o")(axiomNamespace), refType)
-      val field = LocalVarDecl(Identifier("f")(axiomNamespace), fieldType)
-      val args = staticMask ++ Seq(obj, field)
-      val funcApp = FuncApp(hasDirectPermName, args map (_.l), Bool)
-      val permission = currentPermission(staticMask(0).l, obj.l, field.l)
-      Func(hasDirectPermName, args, Bool) ++
-        Axiom(Forall(
-          staticMask ++ Seq(obj, field),
-          Trigger(funcApp),
-          funcApp <==> permissionPositive(permission)
-        ))
-    } ++ {
-      val obj = LocalVarDecl(Identifier("o")(axiomNamespace), refType)
-      val field = LocalVarDecl(Identifier("f")(axiomNamespace), fieldType)
-      val args = Seq(resultMask,summandMask1,summandMask2)
-      val funcApp = FuncApp(sumMasks, args map (_.l), Bool)
-      val permResult = currentPermission(resultMask.l, obj.l, field.l)
-      val permSummand1 = currentPermission(summandMask1.l,obj.l,field.l)
-      val permSummand2 = currentPermission(summandMask2.l,obj.l,field.l)
-      Func(sumMasks,args,Bool) ++
-        Axiom(Forall(
-          args++Seq(obj,field),
-          Trigger(Seq(funcApp,permResult)) ++ Trigger(Seq(funcApp,permSummand1)) ++
-            Trigger(Seq(funcApp,permSummand2)),
-          funcApp ==> (permResult === (permSummand1 + permSummand2))
-        ))
-    } ++ {
-      MaybeCommentedDecl("Function for trigger used in checks which are never triggered",
-        triggerFuncs)
-    } ++ {
-      MaybeCommentedDecl("Functions used as inverse of receiver expressions in quantified permissions during inhale and exhale",
-        inverseFuncs)
-    } ++ {
-      MaybeCommentedDecl("Functions used to represent the range of the projection of each QP instance onto its receiver expressions for quantified permissions during inhale and exhale",
-        rangeFuncs)
+      {
+        MaybeCommentedDecl("Function for trigger used in checks which are never triggered",
+          triggerFuncs)
+      } ++ {
+        MaybeCommentedDecl("Functions used as inverse of receiver expressions in quantified permissions during inhale and exhale",
+          inverseFuncs)
+      } ++ {
+        MaybeCommentedDecl("Functions used to represent the range of the projection of each QP instance onto its receiver expressions for quantified permissions during inhale and exhale",
+          rangeFuncs)
+      }
     }
   }
-
+ 
   def permType = NamedType(permTypeName)
 
   def staticStateContributions(withHeap: Boolean, withPermissions: Boolean): Seq[LocalVarDecl] = if (withPermissions) Seq(LocalVarDecl(maskName, maskType)) else Seq()
@@ -333,6 +411,9 @@ class QuantifiedPermModule(val verifier: Verifier)
    * optimize the check if possible.
    */
   override def permissionPositive(permission: Exp, zeroOK : Boolean = false): Exp = permissionPositiveInternal(permission, None, zeroOK)
+  def permissionFull: Exp = fst(fullPerm, Real) === RealLit(1) && (snd(fullPerm, Bool) === FalseLit())
+  def permissionNo: Exp = (fst(noPerm, Real) === RealLit(0)) && (snd(noPerm, Bool) === FalseLit())
+
 
   private def permissionPositiveInternal(permission: Exp, silPerm: Option[sil.Exp] = None, zeroOK : Boolean = false): Exp = {
     (permission, silPerm) match {
@@ -340,7 +421,7 @@ class QuantifiedPermModule(val verifier: Verifier)
       case (_, Some(sil.FullPerm())) => TrueLit()
       case (_, Some(sil.WildcardPerm())) => TrueLit()
       case (_, Some(sil.NoPerm())) => if (zeroOK) TrueLit() else FalseLit()
-      case _ => if(zeroOK) permission >= noPerm else permission > noPerm
+      case _ => if(zeroOK) fst(permission, Real) >= fst(noPerm, Real) else fst(permission, Real) > fst(noPerm, Real)
     }
   }
 
@@ -362,9 +443,8 @@ class QuantifiedPermModule(val verifier: Verifier)
         val p = PermissionSplitter.normalizePerm(prm)
         val perms = PermissionSplitter.splitPerm(p) filter (x => x._1 - 1 == exhaleModule.currentPhaseId)
         (if (exhaleModule.currentPhaseId == 0)
-          (if (!p.isInstanceOf[sil.WildcardPerm] && !p.isInstanceOf[sil.SWildcardPerm])
-            Assert(permissionPositiveInternal(translatePerm(p), Some(p), true), error.dueTo(reasons.NegativePermission(p)))
-          else Nil: Stmt) ++ Nil // check amount is non-negative
+          (if (!p.isInstanceOf[sil.WildcardPerm])
+            Assert(permissionPositiveInternal(translatePerm(p), Some(p), true), error.dueTo(reasons.NegativePermission(p))) else Nil: Stmt) ++ Nil // check amount is non-negative
         else Nil) ++
           (if (perms.size == 0) {
             Nil
@@ -377,9 +457,6 @@ class QuantifiedPermModule(val verifier: Verifier)
                 val (permVal, wildcard, stmts): (Exp, Exp, Stmt) =
                   if (perm.isInstanceOf[sil.WildcardPerm]) {
                     val w = LocalVar(Identifier("wildcard"), Real)
-                    (w, w, LocalVarWhereDecl(w.name, w > noPerm) :: Havoc(w) :: Nil)
-                  } else if (perm.isInstanceOf[sil.SWildcardPerm]) {
-                    val w = LocalVar(Identifier("sWildcard"), Real)
                     (w, w, LocalVarWhereDecl(w.name, w > noPerm) :: Havoc(w) :: Nil)
                   } else {
                     onlyWildcard = false
@@ -856,9 +933,6 @@ class QuantifiedPermModule(val verifier: Verifier)
           if (perm.isInstanceOf[WildcardPerm]) {
             val w = LocalVar(Identifier("wildcard"), Real)
             (w, LocalVarWhereDecl(w.name, w > noPerm) :: Havoc(w) :: Nil)
-          } else if (perm.isInstanceOf[SWildcardPerm]) {
-            val w = LocalVar(Identifier("sWildcard"), Real)
-            (w, LocalVarWhereDecl(w.name, w > noPerm) :: Havoc(w) :: Nil)
           } else {
             (translatePerm(perm), Nil)
           }
@@ -926,7 +1000,6 @@ class QuantifiedPermModule(val verifier: Verifier)
        checks if the set of expressions conforms to a valid trigger in Boogie:
        - A matching pattern/expression must be more than just a variable by itself
        - only contains permitted types of expressions
-
    */
   def validTrigger(vars:Seq[LocalVarDecl], exps:Seq[Exp]) : Boolean = {
     varMap = Map()
@@ -1254,7 +1327,6 @@ class QuantifiedPermModule(val verifier: Verifier)
   override def transferAdd(e:TransferableEntity, cond:Exp): Stmt = {
     val curPerm = currentPermission(e.rcv,e.loc)
     /* GP: probably redundant in current transfer as these assumputions are implied
-
       (cond := cond && permissionPositive(e.transferAmount, None,true)) ++
       {
       e match {
@@ -1307,8 +1379,6 @@ class QuantifiedPermModule(val verifier: Verifier)
         fullPerm
       case sil.WildcardPerm() =>
         sys.error("cannot translate wildcard at an arbitrary position (should only occur directly in an accessibility predicate)")
-      case sil.SWildcardPerm() =>
-        sys.error((e isSubtype sil.Perm)+"cannot translate wildcard at an arbitrary position (should only occur directly in an accessibility predicate)")
       case sil.EpsilonPerm() =>
         sys.error("epsilon permissions are not supported by this permission module")
       case sil.CurrentPerm(loc: LocationAccess) =>
